theories/compiler/compiler.v
@@ -1,0 +1,91 @@
+Require Export refframe.module.
+Require Import refframe.trefines.
+Require Import refframe.filter.
+Require Import refframe.product.
+Require Import refframe.seq_product.
+Require Import refframe.link.
+Require Import refframe.prepost.
+Require Import refframe.proof_techniques.
+Require Import refframe.imp.
+Require Import refframe.asm.
+Require Import refframe.imp_to_asm.
+Require Import refframe.compiler.monad.
+Require Import refframe.compiler.linear_imp.
+Require Import refframe.compiler.ssa.
+Require Import refframe.compiler.linearize.
+Require Import refframe.compiler.codegen.
+
+Local Open Scope Z_scope.
+Set Default Proof Using "Type".
+
+Inductive compile_error :=
+| LinearizeError (e : ci2a_linearize.error)
+| CodegenError (e : ci2a_codegen.error)
+.
+
+Definition compile_ssa (fn : fndef) : static_fndef :=
+  let static := fndef_to_static_fndef fn in
+  ci2a_ssa.pass_fn static.
+
+Definition compile_linear (fn : fndef) : compiler_success compile_error lfndef :=
+  let ssa := compile_ssa fn in
+  compiler_success_fmap_error LinearizeError (ci2a_linearize.pass_fn ssa).
+
+Definition compile (f2i : gmap string Z) (fn : fndef) : compiler_success compile_error (list deep_asm_instr) :=
+  linear ← compile_linear fn;
+  compiler_success_fmap_error CodegenError (ci2a_codegen.pass_fn f2i linear).
+
+Lemma compile_correct f2i f fn dins ins a:
+  compile f2i fn = CSuccess dins →
+  ins = deep_to_asm_instrs a dins →
+  f2i !! f = Some a →
+  (∀ f' i', f2i !! f' = Some i' → ins !! i' = None ↔ f' ≠ f) →
+  trefines (MS asm_module (initial_asm_state ins))
+           (MS (imp_to_asm (dom _ ins) {[f]} f2i imp_module)
+               (initial_imp_to_asm_state imp_module (initial_imp_state (<[f := fn]> ∅)))).
+Proof.
+  unfold compile.
+  move => /compiler_success_bind_success[?[/compiler_success_fmap_error_success ? /compiler_success_fmap_error_success?]].
+  move => ??.
+  etrans. {
+    apply: ci2a_codegen.pass_fn_correct; [done..| |done].
+    admit.
+  }
+  apply imp_to_asm_trefines; [apply _|].
+  etrans. {
+    apply: ci2a_linearize.pass_fn_correct; [done|..]; rewrite ci2a_ssa.pass_fn_vars.
+    - admit.
+    - admit.
+  }
+  etrans. { apply: ci2a_ssa.pass_fn_correct. }
+  rewrite /initial_imp_sstate fmap_insert fmap_empty static_fndef_to_fndef_to_static_fndef.
+  done.
+Admitted.
+
+Module ci2a_test.
+
+Definition test_fn_1 : fndef := {|
+  fd_args := ["x"];
+  fd_body := (BinOp (BinOp (Var "x") ShiftOp (Val 2)) AddOp (Call "f" [Load (Var "x"); Val 1]));
+  fd_static := I;
+|}.
+
+Compute compile_ssa test_fn_1.
+Compute compile_linear test_fn_1.
+Compute compile (<["f" := 100]> ∅) test_fn_1.
+
+Definition test_sum : fndef := {|
+  fd_args := ["n"];
+  fd_body :=
+    If (BinOp (Var "n") EqOp (Val 0)) (
+         (Val 0)
+    ) (
+       LetE "rec" (Call "sum" [BinOp (Var "n") AddOp (Val (-1))]) $
+       BinOp (Var "n") AddOp (Var "rec"));
+  fd_static := I;
+|}.
+
+Compute compile_ssa test_sum.
+Compute compile_linear test_sum.
+Compute compile (<["sum" := 100]> ∅) test_sum.
+End ci2a_test.
