theories/compiler/ssa.v
@@ -1,0 +1,200 @@
+Require Export refframe.module.
+Require Import refframe.trefines.
+Require Import refframe.filter.
+Require Import refframe.product.
+Require Import refframe.seq_product.
+Require Import refframe.link.
+Require Import stdpp.pretty.
+Require Import refframe.prepost.
+Require Import refframe.proof_techniques.
+Require Import refframe.imp.
+
+Local Open Scope Z_scope.
+Set Default Proof Using "Type".
+
+Definition ssa_var (s : string) (n : N) : string :=
+  s ++ "$" ++ pretty n.
+
+Global Instance ssa_var_inj : Inj2 (=) (=) (=) ssa_var.
+Proof.
+  move => ????. unfold ssa_var => ?. simplify_eq.
+Admitted.
+
+Module ci2a_ssa.
+
+Fixpoint state_bind {S A} (l : list (S → (S * A))) (s : S) : (S * list A) :=
+  match l with
+  | [] => (s, [])
+  | f::l' =>
+      let r1 := f s in
+      let r2 := state_bind l' r1.1 in
+      (r2.1, r1.2::r2.2)
+  end.
+
+Fixpoint pass (ren : gmap string string) (e : static_expr) (s : N) : (N * static_expr) :=
+  match e with
+  | SVar v => (s, SVar (default v (ren !! v)))
+  | SVal v => (s, SVal v)
+  | SBinOp e1 o e2 =>
+      let p1 := pass ren e1 s in
+      let p2 := pass ren e2 p1.1 in
+      (p2.1, SBinOp p1.2 o p2.2)
+  | SAlloc e1 =>
+      let p1 := pass ren e1 s in
+      (p1.1, SAlloc p1.2)
+  | SFree e1 =>
+      let p1 := pass ren e1 s in
+      (p1.1, SFree p1.2)
+  | SLoad e1 =>
+      let p1 := pass ren e1 s in
+      (p1.1, SLoad p1.2)
+  | SStore e1 e2 =>
+      let p1 := pass ren e1 s in
+      let p2 := pass ren e2 p1.1 in
+      (p2.1, SStore p1.2 p2.2)
+  | SCall f args =>
+      let p1 := state_bind (pass ren <$> args) s in
+      (p1.1, SCall f p1.2)
+  | SUbE => (s, SUbE)
+  | SLetE v e1 e2 =>
+      let p1 := pass ren e1 (s + 1) in
+      let p2 := pass (<[v := ssa_var v s]> ren) e2 p1.1 in
+      (p2.1, SLetE (ssa_var v s) p1.2 p2.2)
+  | SIf e1 e2 e3 =>
+      let p1 := pass ren e1 s in
+      let p2 := pass ren e2 p1.1 in
+      let p3 := pass ren e3 p2.1 in
+      (p3.1, SIf p1.2 p2.2 p3.2)
+  end.
+
+Definition test_fn_1 : fndef := {|
+  fd_args := ["x"];
+  fd_body := (LetE "x" (LetE "x" (Var "x") $ Var "x") $
+              LetE "y" (Var "x") $
+              LetE "x" (Var "x") $
+              Var "x");
+  fd_static := I;
+|}.
+Compute (pass ∅ (expr_to_static_expr $ test_fn_1.(fd_body)) 0).
+
+Lemma pass_state ren s e :
+  (pass ren e s).1 = (s + N.of_nat (length (assigned_vars (static_expr_to_expr e))))%N.
+Proof.
+  revert ren s. induction e => //= ren s; try lia.
+  all: rewrite ?IHe1 ?IHe2 ?IHe3 ?app_length; try lia.
+  move: ren s.
+  revert select (Forall _ _). elim; csimpl; [lia|].
+  move => ?? IH1 _ IH2 ??. rewrite IH1 IH2 app_length. lia.
+Qed.
+
+Lemma pass_vars ren s e :
+  assigned_vars (static_expr_to_expr (pass ren e s).2) =
+  imap (λ n v, ssa_var v (s + N.of_nat n)) (assigned_vars (static_expr_to_expr e)).
+Proof.
+  revert ren s. induction e => //= ren s.
+  all: rewrite ?IHe1 ?IHe2 ?IHe3 ?pass_state ?imap_app.
+  all: repeat match goal with
+              | |- _ :: _ = _ :: _ => f_equal
+              | |- _ ++ _ = _ ++ _ => f_equal
+              | |- imap _ _ = imap _ _ => apply imap_ext => * /=
+              | |- ssa_var _ _ = ssa_var _ _ => f_equal
+              end; try lia.
+Admitted.
+
+Lemma pass_correct Ki Ks ei es es' n h fns1 fns2 s vsi vss ren
+      `{!ImpExprFill es Ks (subst_map vss (static_expr_to_expr es'))}
+      `{!ImpExprFill ei Ki (subst_map vsi (static_expr_to_expr (pass ren es' s).2))}:
+  imp_proof_call n fns1 fns2 →
+  (∀ i v, vss !! i = Some v → ∃ i', ren !! i = Some i' ∧ vsi !! i' = Some v) →
+  (∀ x s', (s ≤ s')%N → vsi !! ssa_var x s' = None) →
+  (∀ h' v',
+    Imp (expr_fill Ki $ (Val v')) h' fns1
+       ⪯{imp_module, imp_module, n, false}
+    Imp (expr_fill Ks (Val v')) h' fns2) →
+  Imp ei h fns1
+      ⪯{imp_module, imp_module, n, false}
+  Imp es h fns2.
+Proof.
+  move => Hcall.
+  revert es ei ren s vsi vss h Ks Ki ImpExprFill0 ImpExprFill1.
+  induction es' => //= es ei ren s vsi vss h Ks Ki [?] [?] Hvs Hvars Hcont; simplify_eq.
+  - destruct (vss !! x) eqn: Hx. 2: by tstep_s.
+    move: Hx => /Hvs[?[-> ->]]. done.
+  - done.
+  - apply: IHes'1; [eauto_tstep|eauto_tstep|done|done|] => /= ??.
+    apply: IHes'2; [eauto_tstep|eauto_tstep|done|rewrite pass_state;naive_solver lia|] => /= ??.
+    tstep_s => ??. tstep_i. split!. by apply tsim_mono_b_false.
+  - apply: IHes'; [eauto_tstep|eauto_tstep|done|done|] => /= ??.
+    tstep_s => *. subst. tstep_i. split!. by apply tsim_mono_b_false.
+  - apply: IHes'1; [eauto_tstep|eauto_tstep|done|done|] => /= ??.
+    apply: IHes'2; [eauto_tstep|eauto_tstep|done|rewrite pass_state;naive_solver lia|] => /= ??.
+    tstep_s => *. subst. tstep_i. split!. by apply tsim_mono_b_false.
+  - apply: IHes'; [eauto_tstep|eauto_tstep|done|done|] => /= ??.
+    admit.
+  - apply: IHes'; [eauto_tstep|eauto_tstep|done|done|] => /= ??.
+    tstep_s => *. subst. tstep_i. split!. by apply tsim_mono_b_false.
+  - apply: IHes'1; [eauto_tstep|eauto_tstep|done|done|] => /= ??.
+    tstep_s => *. subst. tstep_i. apply tsim_mono_b_false. case_match.
+    + apply: IHes'2; [eauto_tstep|eauto_tstep|done|rewrite pass_state;naive_solver lia|] => /= ??. done.
+    + apply: IHes'3; [eauto_tstep|eauto_tstep|done|rewrite !pass_state;naive_solver lia|] => /= ??. done.
+  - apply: IHes'1; [eauto_tstep|eauto_tstep|done|naive_solver lia|] => /= ??.
+    tstep_i. tstep_s. rewrite -!subst_subst_map_delete. apply tsim_mono_b_false.
+    apply: IHes'2; [eauto_tstep|eauto_tstep| | |done].
+    + move => ?? /lookup_insert_Some[[??]|[?/Hvs[?[? Hvsi]]]]; simplify_eq.
+      { eexists _. by simplify_map_eq. }
+      eexists _. rewrite lookup_insert_ne //. split; [done|].
+      apply lookup_insert_Some. right. split!. move => ?. subst. move: Hvsi.
+      apply: eq_None_ne_Some_1. naive_solver lia.
+    + move => ? s'. rewrite !pass_state => ?. apply lookup_insert_None. naive_solver lia.
+  - rewrite -(app_nil_l (subst_map vsi <$> _)) -(app_nil_l (subst_map vss <$> _)).
+    change ([]) with (Val <$> []). move: [] => vs. move: s vs h Hvars.
+    revert select (Forall _ _). elim.
+    + move => ???? /=. rewrite app_nil_r.
+      apply: Hcall; [eauto_tstep|eauto_tstep|done| | |done|done|done].
+      { apply Forall2_fmap_l. apply Forall_Forall2_diag. by apply Forall_true. }
+      { apply Forall2_fmap_l. apply Forall_Forall2_diag. by apply Forall_true. }
+    + move => ?? IH _ IH2 s vs h Hvars. csimpl.
+      eapply IH; [| |done|done|] => /=.
+      { constructor. by instantiate (1:=(CallCtx _ _ _) ::_). }
+      { constructor. by instantiate (1:=(CallCtx _ _ _) ::_). }
+      move => ?? /=. rewrite !cons_middle !app_assoc -fmap_snoc. apply IH2.
+      rewrite pass_state. naive_solver lia.
+  - by tstep_s.
+Admitted.
+
+Definition pass_fn (f : static_fndef) : static_fndef :=
+  let args := imap (λ n v, ssa_var v (N.of_nat n)) f.(sfd_args) in
+  {|
+     sfd_args := args;
+     sfd_body := (pass (list_to_map (zip f.(sfd_args) args)) f.(sfd_body) (N.of_nat (length f.(sfd_args)))).2;
+  |}.
+
+Compute pass_fn (fndef_to_static_fndef test_fn_1).
+
+Lemma pass_fn_vars f :
+  sfd_args (pass_fn f) ++ assigned_vars (static_expr_to_expr (sfd_body (pass_fn f))) =
+  imap (λ n v, ssa_var v (N.of_nat n)) (sfd_args f ++ assigned_vars (static_expr_to_expr (sfd_body f))).
+Proof.
+  rewrite imap_app. f_equal => /=. rewrite pass_vars.
+  apply imap_ext. move => *. f_equal. lia.
+Qed.
+
+Lemma pass_fn_correct f fn :
+  trefines (MS imp_module (initial_imp_sstate (<[f := pass_fn fn]> ∅)))
+           (MS imp_module (initial_imp_sstate (<[f := fn]> ∅))).
+Proof.
+  apply imp_proof. { move => ?. rewrite !lookup_fmap !fmap_None !lookup_insert_None. naive_solver. }
+  move => ???????. rewrite !fmap_insert !fmap_empty /=.
+  move => /lookup_insert_Some[[??]|[??]]; simplify_map_eq. split!. { by rewrite imap_length. }
+  rewrite imap_length. move => ?? Hret.
+  rewrite !subst_l_subst_map; [|rewrite ?imap_length; lia..].
+  apply: pass_correct; [eauto_tstep|eauto_tstep|done|..].
+  - move => i v Hl.
+    admit.
+  - move => ???. apply not_elem_of_list_to_map_1.
+    move => /elem_of_list_fmap[[??][?]] /(elem_of_zip_with _ _ _ _)[?[?[?[/elem_of_lookup_imap]]]].
+    move => [?[?[? /(lookup_lt_Some _ _ _) ?]]]. naive_solver lia.
+  - move => ?? /=. by apply Hret.
+Admitted.
+
+End ci2a_ssa.
